src/tls/ECGroup.fst
@@ -1,62 +1,75 @@
 module ECGroup
 
-open FStar.Bytes
 open FStar.Error
-open CoreCrypto
-
 open TLSError
 open Mem
 open Parse
 
-module CC = CoreCrypto
+module B = FStar.Bytes
+module LB = LowStar.Buffer
+module EC = EverCrypt
 module LP = LowParse.SLow.Base
 
-type params = CC.ec_params
-
 type ec_all_curve =
-  | EC_CORE of ec_curve
-  | EC_UNKNOWN of (n:nat{repr_bytes n <= 2})
+  | EC_CORE of group
+  | EC_UNKNOWN of (n:nat{B.repr_bytes n <= 2})
   | EC_EXPLICIT_PRIME
   | EC_EXPLICIT_BINARY
 
-val params_of_group: group -> bool -> Tot params
-let params_of_group c compression = {curve = c; point_compression = compression}
+// FIXME eqtype is a lie but the idealization needs equality of keyshares
+let _key g = assume false; EC.ecdh_state
 
 let pubshare #g k =
-  match g with
-  | ECC_X25519 ->
-    let KS_X25519 ks = k in S_X25519 (TLS.Curve25519.pubshare ks)
-  | ECC_X448 ->
-    let KS_X448 (p,s) = k in S_X448 p
-  | _ ->
-    let KS_CC ks = k in S_CC ks.ec_point
+  match k with
+  | KS_CC p _ -> S_CC p
+  | KS_X25519 k -> S_X25519 (TLS.Curve25519.pubshare k)
+  | KS_X448 p _ -> S_X448 p
 
 #reset-options "--using_facts_from '* -LowParse'"
 let keygen g =
   match g with
-  | ECC_X25519 -> KS_X25519 (TLS.Curve25519.keygen ())
-  | ECC_X448 ->
+  | EverCrypt.ECC_X25519 -> KS_X25519 (TLS.Curve25519.keygen ())
+  | EverCrypt.ECC_X448 ->
     let s = Random.sample32 56ul in
     let p = Random.sample32 56ul in
-    KS_X448 (p, s)
+    KS_X448 p s
   | _ ->
-    let params = params_of_group g false in
-    let s = ec_gen_key params in
-    KS_CC s
+    push_frame ();
+    let l = FStar.UInt32.uint_to_t (bytelen g) in
+    let xb = LB.alloca 0uy l in
+    let yb = LB.alloca 0uy l in
+    assume false; // FIXME EverCrypt framing
+    let st = EC.ecdh_load_curve g in
+    EC.ecdh_keygen st xb yb;
+    let p : point g = { ecx = B.of_buffer l xb; ecy = B.of_buffer l yb } in
+    pop_frame ();
+    KS_CC p st
 
 let dh_initiator #g gx gy =
   match g with
-  | ECC_X25519 ->
+  | EverCrypt.ECC_X25519 ->
     let KS_X25519 (p,s) = gx in
     let S_X25519 gy = gy in
     TLS.Curve25519.mul s gy
-  | ECC_X448 ->
-    let KS_X448 (p,s) = gx in
+  | EverCrypt.ECC_X448 ->
+    let KS_X448 p s = gx in
     s // TODO BEWARE
   | _ ->
-    let KS_CC gx = gx in
+    let KS_CC _ st = gx in
     let S_CC gy = gy in
-    ecdh_agreement gx gy
+    push_frame ();
+    let l = UInt32.uint_to_t (bytelen g) in
+    let xb = LB.alloca 0uy l in
+    let yb = LB.alloca 0uy l in
+    let rb = LB.alloca 0uy l in
+    B.store_bytes gy.ecx xb;
+    B.store_bytes gy.ecy yb;
+    assume false; // FIXME EverCrypt framing
+    let ol = EC.ecdh_compute st xb yb rb in
+    let r = B.of_buffer ol rb in
+    EC.ecdh_free_curve st;
+    pop_frame (); r
+    
 #reset-options
 
 // cwinter: parse_curve, parse_point, and parse_partial really describe
@@ -65,20 +78,20 @@ let dh_initiator #g gx gy =
 // but I can't figure out whether that type has a name in the RFCs
 // (I don't think so, because 'namedcurve' in ECParameters only contains the 
 // curve name, no further parameters).
-val parse_curve: bytes -> Tot (option group)
+val parse_curve: B.bytes -> Tot (option group)
 let parse_curve b =
-  if (length b < 1) then None else (
+  if (B.length b < 1) then None else (
     let open Format.ECCurveType in  
     let open Format.NamedGroup in
     match ecCurveType_parser32 b with // <- parse_curve == ecCurveType_parser and-then named_group_parser
     | Some (Format.ECCurveType.NAMED_CURVE, _) -> 
-      let ty, id = split b 1ul in
+      let ty, id = B.split b 1ul in
       (match namedGroup_parser32 id with
-       | Some (SECP256R1, _) -> Some CC.ECC_P256
-       | Some (SECP384R1, _) -> Some CC.ECC_P384
-       | Some (SECP521R1, _) -> Some CC.ECC_P521
-       | Some (X25519, _   ) -> Some CC.ECC_X25519
-       | Some (X448, _     ) -> Some CC.ECC_X448
+       | Some (SECP256R1, _) -> Some EC.ECC_P256
+       | Some (SECP384R1, _) -> Some EC.ECC_P384
+       | Some (SECP521R1, _) -> Some EC.ECC_P521
+       | Some (X25519, _   ) -> Some EC.ECC_X25519
+       | Some (X448, _     ) -> Some EC.ECC_X448
        | _                   -> None)
     | _ -> None)
 
@@ -86,25 +99,22 @@ let parse_curve b =
 let parse_point g b =
   // parser for flat bytes or uncompressedPointPepresentation
   match g with
-  | ECC_X448 -> (
+  | EC.ECC_X448 -> (
       let (p:LP.parser32 _) = LowParse.SLow.parse32_flbytes 56 56ul in
       match p b with
       | Some (bs, _) -> Some (S_X448 bs)
       | _ -> None)
-  | ECC_X25519 -> (
+  | EC.ECC_X25519 -> (
       let (p:LP.parser32 _) = LowParse.SLow.parse32_flbytes 32 32ul in
       match p b with
       | Some (bs, _) -> Some (S_X25519 bs)
       | _ -> None)
   | _ ->
       let open Format.UncompressedPointRepresentation in
-      let cl = UInt32.uint_to_t (ec_bytelen g) in
+      let cl = UInt32.uint_to_t (bytelen g) in
       match (uncompressedPointRepresentation_parser32 cl) b with
       | Some (ucpr, _) -> 
-          let e = { ecx = ucpr.x; ecy = ucpr.y } in
-          if CoreCrypto.ec_is_on_curve (params_of_group g false) e then
-            Some (S_CC e)
-          else None
+          let e = { ecx = ucpr.x; ecy = ucpr.y } in Some (S_CC e)
     | _ -> None
 
 let parse_partial payload =
@@ -113,8 +123,8 @@ let parse_partial payload =
     // namedGroup_parser (or NamedCurve) and-then
     // ( uncompressedPointRepresentation_parser or flbytes_parser )
     // We should rewrite it using parser combinators
-    if length payload >= 7 then
-      let (curve, point) = split payload 3ul in
+    if B.length payload >= 7 then
+      let (curve, point) = B.split payload 3ul in
       match parse_curve curve with
       | None -> Error(AD_decode_error, perror __SOURCE_FILE__ __LINE__ "Unsupported curve")
       | Some(ecp) ->
@@ -133,44 +143,44 @@ open FStar.Mul
 (* Assumes uncompressed point format for now (04||ecx||ecy) *)
 let serialize_point #g s =
   match g with
-  | ECC_X25519 ->
+  | EC.ECC_X25519 ->
     let S_X25519 p = s in     
-    let r = LowParse.SLow.serialize32_flbytes (ec_bytelen g) p in
-    assume (length r = ec_bytelen g);
+    let r = LowParse.SLow.serialize32_flbytes (bytelen g) p in
+    assume (B.length r = bytelen g);
     r
-  | ECC_X448 ->
+  | EC.ECC_X448 ->
     let S_X448 p = s in    
-    let r = LowParse.SLow.serialize32_flbytes (ec_bytelen g) p in
-    assume (length r = ec_bytelen g);
+    let r = LowParse.SLow.serialize32_flbytes (bytelen g) p in
+    assume (B.length r = bytelen g);
     r
   | _ ->
     let S_CC e = s in
     let open Format.UncompressedPointRepresentation in    
-    let l = length e.ecx in
+    let l = B.length e.ecx in
     let (l32:coordinate_length_type) = UInt32.uint_to_t l in
     let (ucp:uncompressedPointRepresentation l32) = { legacy_form = 4uy; x = e.ecx; y = e.ecy } in
     let x = (uncompressedPointRepresentation_serializer32 l32) ucp in
-    assume (length x = 2 * (ec_bytelen g) + 1);
+    assume (B.length x = 2 * (bytelen g) + 1);
     x
 
-let curve_id g : Tot (lbytes 2) =
+let curve_id g : Tot (B.lbytes 2) =
   let open Format.NamedGroup in
   let r = namedGroup_serializer32 ( // <- curve_id == namedGroup_serializer
     match g with
-    | ECC_P256   -> SECP256R1
-    | ECC_P384   -> SECP384R1
-    | ECC_P521   -> SECP521R1
-    | ECC_X25519 -> X25519
-    | ECC_X448   -> X448) in
-  assume (length r = 2);
+    | EC.ECC_P256   -> SECP256R1
+    | EC.ECC_P384   -> SECP384R1
+    | EC.ECC_P521   -> SECP521R1
+    | EC.ECC_X25519 -> X25519
+    | EC.ECC_X448   -> X448) in
+  assume (B.length r = 2);
   r
 
 let serialize #g ecdh_Y =
-  // Similar to parse_partial, we should rewrite this using serializer combinators
+  let open FStar.Bytes in
   let ty = abyte 3z in
   let id = curve_id g in
   let e = serialize_point ecdh_Y in
-  lemma_repr_bytes_values (FStar.Bytes.length e);
+  lemma_repr_bytes_values (length e);
   assert (repr_bytes (length e) <= 1);
   let ve = vlbytes 1 e in
   ty @| id @| ve
