src/tls/TLS.Curve25519.fst
@@ -5,6 +5,9 @@ open FStar.Error
 
 open FStar.HyperStack.ST
 
+module B = FStar.Bytes
+module LB = LowStar.Buffer
+
 type scalar = lbytes 32
 type point = lbytes 32
 type keyshare = point * scalar
@@ -13,9 +16,19 @@ let pubshare (k:keyshare) : Tot point = fst k
 
 let scalarmult (secret:Bytes.lbytes 32) (point:Bytes.lbytes 32)
   : ST (lbytes 32)
-       (requires (fun h -> True))
-       (ensures (fun h0 _ h1 -> modifies_none h0 h1)) =
-  EverCrypt.Bytes.x25519 secret point
+  (requires (fun h -> True))
+  (ensures (fun h0 _ h1 -> modifies_none h0 h1)) =
+  push_frame ();
+  let lp = B.len point in
+  let ls = B.len secret in
+  let pb = LB.alloca 0uy lp in
+  let sb = LB.alloca 0uy ls in
+  let out = LB.alloca 0uy 32ul in
+  B.store_bytes point pb;
+  B.store_bytes secret sb;
+  assume false;
+  EverCrypt.x25519 out sb pb;
+  pop_frame (); B.of_buffer 32ul out
 
 let keygen () : ST keyshare
   (requires (fun h0 -> True))
